apc/APCACproof.v
@@ -14,13 +14,14 @@ Module APCAC. Section APCAC.
 
   (* context *)
   Context (md : HMod.t).
-  Context (sp_c sp_a sp_pure : string → option fspec).
+  Context (sp_c sp_a : sp_type).
+  Context (sp_pure : spl_type).
   Context (APCInSpA : sp_incl APCA.Sp sp_a).
-  Context (PureInSpA : sp_sub sp_pure sp_a).
+  Context (PureInSpA : sp_incl sp_pure sp_a).
   Context (PureIsPure :
-            ∀ fn pfsp, 
-            sp_pure fn = Some pfsp 
-            → ∃ scopes, find_body md fn = Some (pure_specbody scopes sp_a pfsp)).
+            ∀ fn pfsp,
+            alist_find (Some fn) sp_pure = Some pfsp
+            → ∃ msk scp, (find_body md fn = Some (pure_specbody sp_a true msk scp pfsp)) ∧ msk APCHdr.apc = true).
 
   Local Definition APCC := (APCC.t sp_c).
   Local Definition APCA := (APCA.t sp_pure sp_a).
@@ -30,7 +31,7 @@ Module APCAC. Section APCAC.
 
   Local Transparent _APC.
 
-  Lemma simF_apc : HSim.sim_fun open APCCMod APCAMod IstFull APCHdr.apc.
+  Lemma simF_apc : HSim.sim_fun open APCCMod APCAMod APCC.init_cond IstFull (Some APCHdr.apc).
   Proof using _crisG PureIsPure PureInSpA APCInSpA.
     init_simF.
     (* init_simF. *)
@@ -44,7 +45,7 @@ Module APCAC. Section APCAC.
     add_ret_l ().
 
     iApply wsim_bind. iSplitL; cycle 1.
-    { iIntros (? ? ? ? ?) "R".
+    { iIntros (? ? ? ? ? ?) "R".
       instantiate (1:=(λ nths '(st_src, _) '(st_tgt, _), IstFull nths st_src st_tgt)%I).
       wsteps_r. force_l. steps_l. forces_l. iSplitR; et. step. iSplit; et. }
 
@@ -63,70 +64,141 @@ Module APCAC. Section APCAC.
     rewrite unfold_APC. steps_r. des_ifs. { step. iFrame. }
     steps_r.
 
-    (* manually do what wsim_unwrapN_tgt does *)
-    unfold unwrapN. des_ifs. 2:{ unfold triggerNB. steps_r. des_ifs. }
-    rename Heq into G, f into q3. steps_r. 
-    
-    (* inlining *)
-    unfold is_Some in *. des. dup grt.
-    apply PureInSpA in grt. rewrite grt in G. inv G; ss.
-    apply PureIsPure in grt1. ss. destruct grt1. unfold find_body in H1.
-    inline_r.
-    { subst FLT. rewrite map_app. apply alist_find_comm.
-      - rewrite map_app. rewrite !map_fst_map_map_snd_refl.
-        apply nodup_comm. rewrite -map_app. eauto.
-      - apply alist_find_app. et.
+    rewrite /is_Some in grt. des.
+    dup PureInSpA. rename PureInSpA0 into PIS.
+    assert (SP: sp_a q1 = x1).
+    { apply PIS; eauto. }
+    rewrite SP. destruct x1; cycle 1.
+    { (* inlining *)
+      hexploit PureIsPure; eauto. i. des. rewrite /find_body in H1. inline_r.
+      { unfold FLT. rewrite map_app. apply alist_find_comm.
+        { rewrite map_app. rewrite !map_fst_map_map_snd_refl.
+          apply nodup_comm. rewrite -map_app. eauto. }
+        { apply alist_find_app. apply H1. }
+      }
+      unfold pure_specbody, SB.sandbox_body, SModTr.trans_ktree, SModTr.trans_body, SModTr.HoareFun.
+      steps_r; ss. rewrite /pure_body /cfunN. hss. steps_r.
+      iDestruct "GRT" as "%"; des; hss.
+
+      (* inlining *)
+      inline_r. force_r q3. steps_r. forces_r. iSplitR; eauto. hss. steps_r.
+      
+      (* normalize itree *)
+      unfold APC at 1. steps_r.
+      
+      (* add meaningleses return in src *)
+      add_ret_l ().
+      iApply wsim_bind. iSplitL; cycle 1.
+      { iIntros (? ? ? ? ? ?) "R". instantiate (1:=(λ nths '(st_src, _) '(st_tgt, _), IstFull nths st_src st_tgt)%I).
+        steps_r. forces_r. iSplitL "GRT"; eauto.
+        steps_r. iApply wsim_reset. iStopProof. eapply H0; et. }
+      steps_r. iApply wsim_reset. iStopProof. eapply H; et.
     }
 
-    unfold pure_specbody, SModTr.trans_ktree, SModTr.HoareFun. steps_r.
-    force_r q4. forces_r. iSplitR "IST"; et.
+    (* inlining *)
+    hexploit PureIsPure; eauto. i. des. rewrite /find_body in H1.
+    steps_r. inline_r.
+    { unfold FLT. rewrite map_app. apply alist_find_comm.
+      { rewrite map_app. rewrite !map_fst_map_map_snd_refl.
+        apply nodup_comm. rewrite -map_app. eauto. }
+      { apply alist_find_app. apply H1. }
+    }
 
-    steps_r. unfold pure_body.
-    (* manually do what wsim_unwrapN_tgt does *)
-    step_r. hss. steps_r. rename q7 into q8, q6 into q7.
-
-    steps_r. iDestruct "GRT" as "%". hss.
+    unfold pure_specbody, SB.sandbox_body, SModTr.trans_ktree, SModTr.trans_body, SModTr.HoareFun. ss.
+    force_r q3. steps_r. force_r (q2↑). steps_r. forces_r. iSplitL "GRT"; eauto.
+    steps_r. rewrite /pure_body /cfunN. hss. steps_r.
+    iDestruct "GRT" as "%"; des; hss.
 
     (* inlining *)
-    inline_r. steps_r. force_r q7. forces_r. iSplitR; et. steps_r.
-
-    (* manually do what wsim_unwrapN_tgt does *)
-    hss. steps_r.
-
+    inline_r. force_r q5. steps_r. forces_r. iSplitR; eauto. hss. steps_r.
+    
     (* normalize itree *)
-    unfold APC at 1.
+    unfold APC at 1. steps_r. 
     
     (* add meaningless return in src *)
     add_ret_l ().
 
     iApply wsim_bind. iSplitL; cycle 1.
-    { iIntros (? ? ? ? ?) "R". instantiate (1:=(λ nths '(st_src, _) '(st_tgt, _), IstFull nths st_src st_tgt)%I).
-      steps_r. forces_r. iSplitL "GRT"; et.
-      steps_r. forces_r. iSplitL "GRT"; et. steps_r. iApply wsim_reset. iStopProof. eapply H0; et. }
+    { iIntros (? ? ? ? ? ?) "R". instantiate (1:=(λ nths '(st_src, _) '(st_tgt, _), IstFull nths st_src st_tgt)%I).
+      steps_r. forces_r. iSplitL "GRT"; eauto.
+      steps_r. force_r (tt↑). steps_r. force_r. iSplitL "GRT"; eauto. steps_r. iApply wsim_reset. iStopProof. eapply H0; et. }
     steps_r. iApply wsim_reset. iStopProof. eapply H; et.
+
     Unshelve. all: ss.
   (*SLOW*)Qed.
 
-  Theorem sim : HSim.t open APCCMod APCAMod emp%I IstFull.
+  Theorem sim : HSim.t open APCCMod APCAMod APCC.init_cond IstFull.
   Proof using _crisG PureIsPure PureInSpA APCInSpA.
-    init_sim.
-    - iIntros "_". iExists [], [], _, _. 
-      iSplit; ss.
-      iSplit; [iSplit|]; eauto.
-      iPureIntro. split; prove_scope.
-    - eapply simF_apc; eauto.
+    eapply hmod_sim_reflR; [hrepeat do 1 unfold_hmod; et | ..]; i.
+    { rewrite /Ist_monotone; eauto. }
+    { prove_sub_perm. }
+    { prove_sub_perm. }
+    { r. hrepeat do 1 unfold_hmod; ss; i. split; eauto.
+      iIntros "_". iSplit; ss. iPureIntro. split; prove_scope. }
+    { eapply HSim.sim_fun_strong. i. rewrite /APCC /APCC.t in H.
+      revert H. unseal CRIS. i; ss; des.
+      { subst. hexploit simF_apc. i. rewrite /APCCMod /APCAMod. eapply simF_apc. }
+      { econs.
+        assert (fn <> Some APCHdr.apc).
+        { ii. subst. inv NODUPFS.
+          { rewrite map_app /APCC /APCC.t in H1. revert H1. unseal CRIS. i; ss. }
+          { rewrite map_app /APCC /APCC.t in H0. revert H0. unseal CRIS. i; ss.
+            inv H0. apply H1. eauto. }
+        }
+        split; eauto.
+        { instantiate (1:=fs).
+          rewrite /APCC /APCC.t in FIND. revert FIND. unseal CRIS. i; ss.
+          des_ifs.
+          { rewrite eq_rel_dec_correct /option_Dec in Heq. des_ifs. }
+          rewrite map_app in NODUPFT. eapply nodup_comm in NODUPFT.
+          rewrite -map_app in NODUPFT.
+          eapply alist_find_comm; eauto.
+          eapply alist_find_app; eauto.
+        }
+        ss. inv WFS. unfold APCC, APCC.t in *. revert_until fn. unseal CRIS. i.
+        destruct fs. do 2 destruct p.
+        hexploit isim_reflR; eauto.
+        { ss. replace ("APC" :: HMod.scopes md) with (["APC"] ++ HMod.scopes md) in wf_scopes by ss.
+          apply wf_scopes. }
+        { instantiate (1:=l). destruct md; ss. des_ifs.
+          { rewrite eq_rel_dec_correct in Heq. des_ifs. }
+          hexploit well_scoped_fns. instantiate (1:=fn).
+          i. rewrite /fnsems_scopes in H1. rewrite FIND in H1. eauto. }
+        { iIntros (??????) "->". eauto. }
+        instantiate (10:=(map (map_snd SB.sandbox_body) (HMod.fnsems (SMod.to_hmod sp_c APCC.Mod) ++ HMod.fnsems md))).
+        instantiate (9:=(map (map_snd SB.sandbox_body) (HMod.fnsems APCA ++ HMod.fnsems md))).
+        instantiate (8:=Ist).
+        instantiate (5:=open).
+        instantiate (2:=(b, b0)).
+        instantiate (1:=f).
+        i. rewrite /HSim.IstS /HSim.IstE.
+        destruct (is_some fn) eqn: E.
+        { unfold APCC.Mod; ss. }
+        rewrite /isim_fsem. i. iIntros "[% INIT]". des; subst.
+        unfold APCC.Mod, APCA, t; ss. unseal CRIS. ss.
+        rewrite /isim_fsem in H1.
+        iApply isim_wand.
+        { instantiate (1:=ist_with_eq (IstProd (IstSB APCC.scopes Ist) IstEq)).
+          iSplitR; eauto.
+          { iIntros (?????) "%". des; subst. eauto. }
+          rewrite /APCA /t in H1. revert H1. unseal CRIS. i.
+          iApply H1; eauto.
+          rewrite /IstProd /IstSB /Ist. iExists [], [], _, _. repeat iSplit; eauto; iPureIntro; ss. }
+      }
+    }
   Qed.
 End APCAC.
 
 Section ctxr.
   Context `{_crisG: !crisG Γ Σ α β τ _S _I}.
 
-  Definition ctxr (md : HMod.t) (sp_c sp_a sp_pure : string → option fspec)
+  Definition ctxr (md : HMod.t) (sp_c sp_a : sp_type) (sp_pure : spl_type)
       (APCInSpA : sp_incl APCA.Sp sp_a)
-      (PureInSpA : sp_sub sp_pure sp_a)
+      (PureInSpA : sp_incl sp_pure sp_a)
       (PureIsPure :
-        ∀ fn pfsp, sp_pure fn = Some pfsp →
-          ∃ scopes, find_body md fn = Some (pure_specbody scopes sp_a pfsp)) :
+        ∀ fn pfsp,
+          alist_find (Some fn) sp_pure = Some pfsp
+          → ∃ msk scp, (find_body md fn = Some (pure_specbody sp_a true msk scp pfsp)) ∧ msk APCHdr.apc = true) :
     ctx_refines
       ((APCC.t sp_c)          ★ md, emp%I)
       ((APCA.t sp_pure sp_a)  ★ md, emp%I).
